more lemmas

theories/logrel/logrel_prim.v
@@ -10,60 +10,54 @@ Section logrel_prim.
   Context `{hypparams:!HypervisorParameters}.
   Context `{vmG: !gen_VMG Σ}.
 
-  Definition trans_rel_primary (i:VMID) (trans trans': gmap Word transaction): Prop :=
-   map_Forall (λ h tran,
-          ((tran.1.1.1.1 ≠ i ∧ tran.1.1.1.2 ≠ i) -> ∃ tran', trans' !! h = Some tran' ∧ tran = tran') ∧
-          ((tran.1.1.1.2 = V0 ∧ tran.2 = true) -> ∃ tran', trans' !! h = Some tran' ∧ tran = tran') ∧
-          ((tran.1.1.1.1 = V0 ∧ tran.1.2 ≠ Donation) -> ∃ tran', trans' !! h = Some tran' ∧ tran.1 = tran'.1)
-     ) trans.
+  (* Definition trans_rel_primary (i:VMID) (trans trans': gmap Word transaction): Prop := *)
+  (*  map_Forall (λ h tran, *)
+  (*         ((tran.1.1.1.1 ≠ i ∧ tran.1.1.1.2 ≠ i) -> ∃ tran', trans' !! h = Some tran' ∧ tran = tran') ∧ *)
+  (*         ((tran.1.1.1.2 = V0 ∧ tran.2 = true) -> ∃ tran', trans' !! h = Some tran' ∧ tran = tran') ∧ *)
+  (*         ((tran.1.1.1.1 = V0 ∧ tran.1.2 ≠ Donation) -> ∃ tran', trans' !! h = Some tran' ∧ tran.1 = tran'.1) *)
+  (*    ) trans. *)
 
-  (* Definition transaction_pagetable_entries_transferred_all (trans: gmap Addr transaction) : iProp Σ:= *)
-  (*   big_sepFM trans (λ kv, kv.2.1.2 = Donation) (λ k v, k -{1/4}>t v.1 ∗ pgt_1_4 v.1.1.2 v.1.1.1.1 true)%I. *)
+  Definition transferred_memory_slice (trans : gmap Addr transaction) (i: VMID) (j:VMID): iProp Σ:=
+     ∃ mem , memory_pages (pages_in_trans (filter (λ kv, (kv.2.1.1.1.1 = i ∧ kv.2.1.1.1.2 = j) ∧ ¬(kv.2.2 = true ∧ kv.2.1.2 = Lending))%type trans)) mem.
 
-  (* Definition retrievable_transaction_transferred_all(trans: gmap Addr transaction) : iProp Σ:= *)
-  (*   (big_sepFM trans (λ kv, True) (λ k v, k -{1/2}>re v.2 )%I) ∗ *)
-  (*   (big_sepFM trans (λ kv, kv.2.2 = false) (λ k v, k -{1/4}>t v.1 ∗ k -{1/2}>re v.2)%I). *)
-
-  (* Definition transaction_pagetable_entries_transferred_except (i: VMID) (trans: gmap Addr transaction) : iProp Σ:= *)
-  (*   big_sepFM trans (λ kv, kv.2.1.2 = Donation ∧ ¬(kv.2.1.1.1.1 = i ∨ kv.2.1.1.1.2 = i)) (λ k v, k -{1/4}>t v.1 ∗ pgt_1_4 v.1.1.2 v.1.1.1.1 true)%I. *)
-
-  (* Definition retrievable_transaction_transferred_except (i: VMID) (trans: gmap Addr transaction) : iProp Σ:= *)
-  (*   (big_sepFM trans (λ kv, ¬(kv.2.1.1.1.1 = i ∨ kv.2.1.1.1.2 = i)) (λ k v, k -{1/2}>re v.2 )%I) ∗ *)
-  (*   (big_sepFM trans (λ kv, ¬(kv.2.1.1.1.1 = i ∨ kv.2.1.1.1.2 = i) ∧ kv.2.2 = false) (λ k v, k -{1/4}>t v.1 ∗ k -{1/2}>re v.2)%I). *)
-
-  (* Definition transferred_memory_pages_all (trans : gmap Word transaction) := *)
-  (*   pages_in_trans (filter (λ kv, ¬(kv.2.2 = true ∧ kv.2.1.2 = Lending)) trans). *)
-
-  Definition transferred_memory_pages_slice (j: VMID) (i:VMID) (trans : gmap Addr transaction) :=
-    pages_in_trans (filter (λ kv, (kv.2.1.1.1.1 = i ∧ kv.2.1.1.1.2 = j) ∧ ¬(kv.2.2 = true ∧ kv.2.1.2 = Lending)) trans).
-
-  Definition retrievable_transaction_transferred_slice (i:VMID) (j: VMID) (trans : gmap Addr transaction) : iProp Σ :=
+  Definition retrievable_transaction_transferred_slice (trans : gmap Addr transaction) (i:VMID) (j: VMID) : iProp Σ :=
     (big_sepFM trans (λ kv, kv.2.1.1.1.1 = i ∧ kv.2.1.1.1.2 = j) (λ k v, k -{1/2}>re v.2 )%I) ∗
     (big_sepFM trans (λ kv, (kv.2.1.1.1.1 = i ∧ kv.2.1.1.1.2 = j) ∧ kv.2.2 = false) (λ k v, k -{1/4}>t v.1 ∗ k -{1/2}>re v.2)%I).
 
-  Definition transaction_pagetable_entries_transferred_slice (i: VMID) (j: VMID) (trans: gmap Addr transaction) : iProp Σ :=
-    big_sepFM trans (λ kv, (kv.2.1.1.1.1 = i ∧ kv.2.1.1.1.2 = j) ∧ kv.2.1.2 = Donation ) (λ k v, k -{1/4}>t v.1 ∗ pgt_1_4 v.1.1.2 v.1.1.1.1 true)%I.
+  Definition transaction_pagetable_entries_transferred_slice (trans: gmap Addr transaction) (i: VMID) (j: VMID) : iProp Σ :=
+    big_sepFM trans (λ kv, (kv.2.1.1.1.1 = i ∧ kv.2.1.1.1.2 = j) ∧ kv.2.1.2 = Donation) (λ k v, k -{1/4}>t v.1 ∗ pgt_1_4 v.1.1.2 v.1.1.1.1 true)%I.
 
   Definition set_of_vmids : gset VMID := (list_to_set list_of_vmids).
 
-  Definition slice_wf (Φ: (gmap Addr transaction) -> (VMID * VMID)-> iProp Σ) :=
-    ∀ i j trans trans', filter (λ kv, kv.2.1.1.1.1 = i ∧ kv.2.1.1.1.2 = j) trans
-                        = filter (λ kv, kv.2.1.1.1.1 = i ∧ kv.2.1.1.1.2 = j) trans' ->
-    (Φ trans (i,j) ⊣⊢ Φ trans' (i,j)).
+  Definition trans_preserve_slice i j (trans trans': (gmap Addr transaction)):=
+    filter (λ kv, kv.2.1.1.1.1 = i ∧ kv.2.1.1.1.2 = j) trans
+                        = filter (λ kv, kv.2.1.1.1.1 = i ∧ kv.2.1.1.1.2 = j) trans'.
 
-  Definition slice_wf2 (Φ: (gmap Addr transaction) -> (VMID * VMID)-> iProp Σ) :=
+  Definition trans_preserve_only i (trans trans': (gmap Addr transaction)) :=
+    filter (λ kv, kv.2.1.1.1.1 = i ∨ kv.2.1.1.1.2 = i) trans
+                        = filter (λ kv, kv.2.1.1.1.1 = i ∨ kv.2.1.1.1.2 = i) trans'.
+
+  (*TODO*)
+  Definition trans_preserve_except i (trans trans': (gmap Addr transaction)) :=
+    map_Forall (λ h tran, ¬(tran.1.1.1.1 = i ∨ tran.1.1.1.2 = i) -> ∃ tran', trans' !! h = Some tran' ∧ tran = tran') trans.
+
+  Definition slice_wf (Φ: (gmap Addr transaction) -> VMID -> VMID -> iProp Σ) :=
+    ∀ i j trans trans', trans_preserve_slice i j trans trans'->
+    (Φ trans i j ⊣⊢ Φ trans' i j).
+
+  Definition slice_wf2 (Φ: (gmap Addr transaction) -> VMID -> VMID -> iProp Σ) :=
     ∀ i j (trans trans' : gmap Addr transaction),
     dom (gset _) (filter (λ kv, kv.2.1.1.1.1 = i ∧ kv.2.1.1.1.2 = j)%type trans') ⊆ dom _ trans ->
     ([∗ map] h ↦ tran ∈ trans, h -{1/2}>t tran.1) ⊢
-    (Φ trans' (i,j)) ∗-∗ (Φ (map_zip (fst<$>trans) (snd <$>trans')) (i,j)).
+    (Φ trans' i j) ∗-∗ (Φ (map_zip (fst<$>trans) (snd <$>trans')) i j).
 
-  Class SliceWf (Φ: (gmap Addr transaction) -> (VMID * VMID)-> iProp Σ):=
+  Class SliceWf (Φ: (gmap Addr transaction) -> VMID -> VMID-> iProp Σ):=
     {
       slice : (slice_wf Φ);
       agree : (slice_wf2 Φ)
     }.
 
-  Program Definition interp_access_prim p_tx p_rx ps_acc trans `(SliceWf Φ): iPropO Σ:=
+  Program Definition interp_access_prim Φ p_tx p_rx ps_acc trans `(!SliceWf Φ): iPropO Σ:=
     (
       (* let ps_macc_trans := (transferred_memory_pages_all trans) in *)
       let ps_oea := ps_acc ∖ {[p_rx;p_tx]} ∖ (currently_accessible_in_trans_memory_pages V0 trans) in
